Move some code from Basic.lean to dedicated files

Bdd/Basic.lean
@@ -732,13 +732,13 @@ def DecisionTree.size {n} : DecisionTree n → Nat
   | leaf _ => 0
   | branch _ l h => 1 + l.size + h.size
 
-def OBdd.size {n m} : OBdd n m → Nat := DecisionTree.size ∘ OBdd.toTree
+def OBdd.size' {n m} : OBdd n m → Nat := DecisionTree.size ∘ OBdd.toTree
 
-lemma OBdd.size_zero_of_terminal : OBdd.isTerminal O → O.size = 0 := by
+lemma OBdd.size_zero_of_terminal : OBdd.isTerminal O → O.size' = 0 := by
   rintro ⟨b, h⟩
   rcases O with ⟨⟨heap, root⟩, o⟩
   subst h
-  simp only [size, Ordered, Function.comp_apply]
+  simp only [size', Ordered, Function.comp_apply]
   unfold toTree
   rfl
 
@@ -756,8 +756,8 @@ lemma OBdd.low_reduced {n m} {O : OBdd n m} {j : Fin m} {h : O.1.root = node j} 
   rw [h]
   exact Edge.low rfl
 
-lemma OBdd.size_node {n m} {O : OBdd n m} {j : Fin m} (h : O.1.root = node j) : O.size = 1 + (O.low h).size + (O.high h).size := by
-  simp only [size, Function.comp_apply, toTree_node h]
+lemma OBdd.size_node {n m} {O : OBdd n m} {j : Fin m} (h : O.1.root = node j) : O.size' = 1 + (O.low h).size' + (O.high h).size' := by
+  simp only [size', Function.comp_apply, toTree_node h]
   rfl
 
 lemma OBdd.evaluate_high_eq_evaluate_low_of_independentOf_root {n m} {O : OBdd n m} {j : Fin m} {h : O.1.root = node j} :
@@ -1001,7 +1001,7 @@ theorem OBdd.HCanonicity {n m m' : Nat} {O : OBdd n m} {U : OBdd n m'}:
       · constructor
         · apply HCanonicity (low_reduced  O_reduced) (low_reduced  U_reduced) (evaluate_low_eq_of_evaluate_eq_and_var_eq'  h same_var)
         · apply HCanonicity (high_reduced O_reduced) (high_reduced U_reduced) (evaluate_high_eq_of_evaluate_eq_and_var_eq' h same_var)
-termination_by O.size + U.size
+termination_by O.size' + U.size'
 decreasing_by
   simp [size_node U_root_def]; linarith
   simp [size_node O_root_def]; linarith
@@ -1038,247 +1038,6 @@ theorem OBdd.Canonicity_reverse {O : OBdd n m} {U : OBdd n m'}:
   simp only [Similar, HSimilar] at h
   simp only [evaluate, Function.comp_apply]
   rw [h]
-
-def OBdd.collect_helper (O : OBdd n m) : Vector Bool m × List (Fin m) → Vector Bool m × List (Fin m) :=
-  match h : O.1.root with
-  | terminal _ => id
-  | node j =>
-    fun I ↦ if I.1.get j then I else collect_helper (O.high h) (collect_helper (O.low h) ⟨I.1.set j true, j :: I.2⟩)
-termination_by O
-
-/-- Return a list of all reachable node indices. -/
-def OBdd.collect : OBdd n m → List (Fin m) :=
-  fun O ↦ (collect_helper O ⟨Vector.replicate m false, []⟩).2
-
-lemma OBdd.collect_helper_terminal {v : Vector (Node n m) m} {h : Bdd.Ordered {heap := v, root := terminal b}} :
-    collect_helper ⟨{heap := v, root := terminal b}, h⟩ I = I := by
-  conv =>
-    lhs
-    unfold collect_helper
-  congr
-
-lemma OBdd.collect_helper_terminal' (O : OBdd n m) (h : O.1.root = terminal b) :
-    collect_helper O I = I := by
-  rcases O with ⟨⟨M, r⟩, o⟩
-  simp only at h
-  have := collect_helper_terminal (h := (show Bdd.Ordered {heap := M, root := terminal b} by simp_rw [← h]; exact o)) (I := I)
-  simp_rw [h]
-  assumption
-
-lemma OBdd.collect_helper_node {v : Vector (Node n m) m} {h : Bdd.Ordered {heap := v, root := node j}} :
-    collect_helper ⟨{heap := v, root := node j}, h⟩ I =
-      if I.1[j]
-      then I
-      else collect_helper ⟨{heap := v, root := v[j].high}, ordered_of_relevant ⟨{heap := v, root := node j}, h⟩ ⟨v[j].high, reachable_of_edge (Edge.high rfl)⟩⟩
-                          (collect_helper ⟨{heap := v, root := v[j].low}, ordered_of_relevant ⟨{heap := v, root := node j}, h⟩ ⟨v[j].low, reachable_of_edge (Edge.low rfl)⟩⟩
-                                          ⟨I.1.set j true, j :: I.2⟩) := by
-  conv =>
-    lhs
-    unfold collect_helper
-  congr
-
-lemma OBdd.collect_helper_node' (O : OBdd n m) {j : Fin m} (h : O.1.root = node j) :
-    collect_helper O I = if I.1[j] then I else collect_helper (O.high h) (collect_helper (O.low h) ⟨I.1.set j true, j :: I.2⟩) := by
-  rcases O with ⟨⟨M, r⟩, o⟩
-  simp only at h
-  have := collect_helper_node (h := (show Bdd.Ordered {heap := M, root := node j} by simp_rw [← h]; exact o)) (I := I)
-  simp_rw [h]
-  assumption
-
-theorem OBdd.collect_helper_retains_found {O : OBdd n m} {I : Vector Bool m × List (Fin m)} :
-    j ∈ I.2 → j ∈ (collect_helper O I).2 := by
-  intro h
-  cases O_root_def : O.1.root with
-  | terminal b =>
-    rw [collect_helper_terminal' O O_root_def]
-    assumption
-  | node i =>
-    rw [collect_helper_node' O O_root_def]
-    cases I.1[i]
-    case true  => simpa
-    case false =>
-      simp only [Bool.false_eq_true, ↓reduceIte]
-      have : j ∈ ((O.low O_root_def).collect_helper (I.1.set i true, i :: I.2)).2 := by
-        apply collect_helper_retains_found
-        simp only []
-        cases decEq j i with
-        | isFalse hf => right; assumption
-        | isTrue ht => rw [ht]; left
-      exact collect_helper_retains_found this
-termination_by O
-
-theorem OBdd.collect_helper_retains_marked {O : OBdd n m} {I : Vector Bool m × List (Fin m)} {j : Fin m}:
-    I.1[j] = true → (collect_helper O I).1[j] = true := by
-  intro h
-  cases O_root_def : O.1.root with
-  | terminal b =>
-    rw [collect_helper_terminal' O O_root_def]
-    assumption
-  | node i =>
-    rw [collect_helper_node' O O_root_def]
-    cases I.1[i]
-    case true  => simpa
-    case false =>
-      simp only [Bool.false_eq_true, ↓reduceIte]
-      have : ((O.low O_root_def).collect_helper (I.1.set i true, i :: I.2)).1[j] = true := by
-        apply collect_helper_retains_marked
-        simp only []
-        cases decEq i j with
-        | isFalse hf =>
-          have : i.1 ≠ j.1 := by
-            exact Fin.val_ne_of_ne hf
-          simp only [Fin.getElem_fin]
-          rw [Vector.getElem_set_ne _ _ this]
-          assumption
-        | isTrue ht => rw [ht]; simp
-      exact collect_helper_retains_marked this
-termination_by O
-
-theorem OBdd.collect_helper_only_marks_reachable {O : OBdd n m} {I : Vector Bool m × List (Fin m)} :
-    I.1[j] = false → (collect_helper O I).1[j] = true → Reachable O.1.heap O.1.root (node j) := by
-  intro h1 h2
-  cases O_root_def : O.1.root with
-  | terminal b =>
-    rw [collect_helper_terminal' O O_root_def, h1] at h2; contradiction
-  | node i =>
-    cases decEq i j with
-    | isTrue ht  => rw [ht]; exact Relation.ReflTransGen.refl
-    | isFalse hf =>
-      rw [collect_helper_node' O O_root_def] at h2
-      cases hh : I.1[i] with
-      | true =>
-        rw [hh] at h2
-        simp only [↓reduceIte] at h2
-        rw [h1] at h2
-        contradiction
-      | false =>
-        rw [hh] at h2
-        simp at h2
-        rw [← O_root_def]
-        cases hhh : ((O.low O_root_def).collect_helper (I.1.set i true, i :: I.2)).1[j] with
-        | false =>
-          have : Reachable (O.high O_root_def).1.heap (O.high O_root_def).1.root (node j) := by
-            apply collect_helper_only_marks_reachable (I := ((O.low O_root_def).collect_helper (I.1.set i true, i :: I.2)))
-            · assumption
-            · assumption
-          simp at this
-          trans (O.high O_root_def).1.root
-          · exact reachable_of_edge (edge_of_high (h := O_root_def) O.1)
-          · assumption
-        | true =>
-          have : Reachable (O.low O_root_def).1.heap (O.low O_root_def).1.root (node j) := by
-            apply collect_helper_only_marks_reachable (I := (I.1.set i true, i :: I.2))
-            · have : i.1 ≠ j.1 := by
-                exact Fin.val_ne_of_ne hf
-              simp only [Fin.getElem_fin]
-              rw [Vector.getElem_set_ne _ _ this]
-              assumption
-            · assumption
-          simp at this
-          trans (O.low O_root_def).1.root
-          · exact reachable_of_edge (edge_of_low (h := O_root_def) O.1)
-          · assumption
-termination_by O
-
-theorem OBdd.collect_helper_spec {O : OBdd n m} :
-    (∀ i, (Reachable O.1.heap O.1.root (node i) → I.1[i] = true → i ∈ I.2)) →
-    ∀ i, (Reachable O.1.heap O.1.root (node i) → (collect_helper O I).1[i] → i ∈ (collect_helper O I).2) := by
-  intro h j re ma
-  cases O_root_def : O.1.root with
-  | terminal b =>
-    have : (⟨node j, re⟩ : O.1.RelevantPointer).1  = terminal b := by
-      apply eq_terminal_of_relevant
-      rw [← O_root_def]
-    contradiction
-  | node k =>
-    rw [collect_helper_node' O O_root_def] at ma
-    rw [collect_helper_node' O O_root_def]
-    cases hh : I.1[k] with
-    | true =>
-      rw [hh] at ma
-      simp at ma
-      simp
-      exact h j re ma
-    | false =>
-      rw [hh] at ma
-      simp at ma
-      simp
-      cases decEq k j with
-      | isTrue hht =>
-        apply collect_helper_retains_found
-        apply collect_helper_retains_found
-        rw [hht]
-        left
-      | isFalse hhf =>
-        cases hhh : I.1[j] with
-        | true =>
-          apply collect_helper_retains_found
-          apply collect_helper_retains_found
-          right
-          apply h <;> assumption
-        | false=>
-          cases hhhh : ((O.low O_root_def).collect_helper (I.1.set k true, k :: I.2)).1[j] with
-          | true =>
-            have : j ∈ ((O.low O_root_def).collect_helper (I.1.set k true, k :: I.2)).2 := by
-              apply collect_helper_spec
-              · intro i' re' ma'
-                simp at ma'
-                simp at re'
-                simp only
-                cases decEq k i' with
-                | isFalse hff =>
-                  rw [Vector.getElem_set_ne _ _ (by simp_all [Fin.val_ne_of_ne hff])] at ma'
-                  right
-                  apply h
-                  exact Reachable.trans (reachable_of_edge (edge_of_low (h := O_root_def) O.1)) re'
-                  exact ma'
-                | isTrue  htt => rw [htt]; left
-              · have : (I.1.set k true, k :: I.2).1[j] = false := by
-                  simp only [Fin.getElem_fin]
-                  rw [Vector.getElem_set_ne _ _ (by simp_all [Fin.val_ne_of_ne hhf])]
-                  exact hhh
-                apply collect_helper_only_marks_reachable this hhhh
-              · exact hhhh
-            apply collect_helper_retains_found this
-          | false=>
-            apply collect_helper_spec
-            · intro i' re' ma'
-              simp at ma' re'
-              have := h i' (Reachable.trans (reachable_of_edge (edge_of_high (h := O_root_def) O.1)) re')
-              cases hhhhh : I.1[i'] with
-              | true =>
-                apply this at hhhhh
-                have : i' ∈ (I.1.set k true, k :: I.2).2 := by simp only; right; exact hhhhh
-                apply collect_helper_retains_found this
-              | false=>
-                cases decEq k i' with
-                | isTrue hhtt =>
-                  apply collect_helper_retains_found
-                  rw [hhtt]
-                  left
-                | isFalse hhff =>
-                  have that : (I.1.set k true, k :: I.2).1[i'] = false := by
-                    simp only [Fin.getElem_fin]
-                    rw [Vector.getElem_set_ne _ _ (by simp_all [Fin.val_ne_of_ne hhff])]
-                    exact hhhhh
-                  apply collect_helper_spec
-                  · intro i'' re'' ma''
-                    simp at ma''
-                    simp at re''
-                    simp only
-                    cases decEq k i'' with
-                    | isFalse hfff =>
-                      rw [Vector.getElem_set_ne _ _ (by simp_all [Fin.val_ne_of_ne hfff])] at ma''
-                      right
-                      apply h
-                      exact Reachable.trans (reachable_of_edge (edge_of_low (h := O_root_def) O.1)) re''
-                      exact ma''
-                    | isTrue  htt => rw [htt]; left
-                  · apply collect_helper_only_marks_reachable that ma'
-                  · exact ma'
-            · apply collect_helper_only_marks_reachable hhhh ma
-            · assumption
-termination_by O
 
 /-- An acyclicity lemma: an edge from `O` to `U` implies that `O` is not reachable from `U`.  -/
 lemma OBdd.not_oedge_reachable {n m} {O U : OBdd n m}: OEdge O U → ¬ Reachable O.1.heap U.1.root O.1.root := by
@@ -1335,7 +1094,6 @@ lemma Pointer.Reachable_iff {M : Vector (Node n m) m } :
         · apply Relation.reflTransGen_swap.mpr; exact h
         · right; rfl
 
-
 lemma OBdd.reachable_or_eq_low_high {O : OBdd n m} :
     Reachable O.1.heap O.1.root p → (O.1.root = p ∨ (∃ j, ∃ (h : O.1.root = node j), (Reachable O.1.heap (O.low h).1.root p ∨ Reachable O.1.heap (O.high h).1.root p))) := by
   intro hr
@@ -1349,247 +1107,10 @@ lemma OBdd.reachable_or_eq_low_high {O : OBdd n m} :
     | inl hl => left;  simpa [low, Bdd.low]
     | inr hh => right; simpa [high, Bdd.high]
 
-lemma OBdd.collect_spec' {O : OBdd n m} {j : Fin m} {I : Vector Bool m × List (Fin m)} :
-    Reachable O.1.heap O.1.root (node j) →
-    (∀ i, (Reachable O.1.heap O.1.root (node i) → Reachable O.1.heap (node i) (node j) → I.1[i] = false)) →
-    (O.collect_helper I).1[j] = true := by
-  intro h1 h2
-  cases O_root_def : O.1.root with
-  | terminal b =>
-    have : (⟨node j, h1⟩ : O.1.RelevantPointer).1  = terminal b := by
-      apply eq_terminal_of_relevant
-      rw [← O_root_def]
-    contradiction
-  | node i =>
-    rw [collect_helper_node' O O_root_def]
-    have : I.1[i] = false := by
-      apply h2 i
-      · rw [← O_root_def]
-        exact Relation.ReflTransGen.refl
-      · rw [← O_root_def]
-        exact h1
-    rw [this]
-    simp only [Bool.false_eq_true, ↓reduceIte]
-    cases decEq i j with
-    | isTrue h =>
-      apply collect_helper_retains_marked
-      apply collect_helper_retains_marked
-      rw [h]
-      simp
-    | isFalse hij =>
-      cases Pointer.instDecidableReachable (O.low O_root_def) (node j) with
-      | isTrue ht  =>
-        apply collect_helper_retains_marked
-        apply collect_spec'
-        · exact ht
-        · intro i' re1 re2
-          simp only
-          cases decEq i i' with
-          | isTrue h =>
-            exfalso
-            apply not_oedge_reachable (oedge_of_low (h := O_root_def))
-            rw [← h] at re1
-            rw [O_root_def]
-            exact re1
-          | isFalse h =>
-            simp only [Fin.getElem_fin]
-            rw [Vector.getElem_set_ne _ _ (by simp_all [Fin.val_ne_of_ne h])]
-            apply h2
-            exact Reachable.trans (reachable_of_edge (edge_of_low (h := O_root_def) O.1)) re1
-            exact re2
-      | isFalse hf =>
-        apply collect_spec'
-        · cases (reachable_or_eq_low_high (p := node j) h1) with
-        | inl h => rw [O_root_def] at h; simp at h; contradiction
-        | inr h =>
-          rcases h with ⟨j', h', d⟩
-          have same : i = j' := by rw [O_root_def] at h'; simp at h'; assumption
-          subst same
-          cases d with
-          | inl => contradiction
-          | inr => assumption
-        · intro i' re ma
-          contrapose! hf
-          simp only [Bool.not_eq_false] at hf
-          apply collect_helper_only_marks_reachable (I := (I.1.set i true, i :: I.2))
-          simp only [Fin.getElem_fin]
-          rw [Vector.getElem_set_ne _ _ (by simp_all [Fin.val_ne_of_ne hij])]
-          apply h2
-          · exact Reachable.trans (reachable_of_edge (edge_of_high (h := O_root_def) O.1)) (Reachable.trans re ma)
-          · exact Relation.ReflTransGen.refl
-          · apply collect_spec'
-            · have that : Reachable (O.low O_root_def).1.heap (O.low O_root_def).1.root (node i') := by
-                apply collect_helper_only_marks_reachable (I := (I.1.set i true, i :: I.2))
-                · cases decEq i i' with
-                  | isFalse hff =>
-                    simp only [Fin.getElem_fin]
-                    rw [Vector.getElem_set_ne _ _ (by simp_all [Fin.val_ne_of_ne hff])]
-                    apply h2 i' (Reachable.trans (reachable_of_edge (edge_of_high (h := O_root_def) O.1)) re) ma
-                  | isTrue htt =>
-                    exfalso
-                    apply not_oedge_reachable (oedge_of_high (h := O_root_def))
-                    rw [htt] at O_root_def
-                    rw [O_root_def]
-                    exact re
-                · assumption
-              exact Reachable.trans that ma
-            · intro i'' re1 re2
-              simp only
-              cases decEq i i'' with
-              | isTrue h =>
-                rw [← h] at re1
-                exfalso
-                apply not_oedge_reachable (oedge_of_low (h := O_root_def))
-                rw [O_root_def]
-                exact re1
-              | isFalse h =>
-                simp only [Fin.getElem_fin]
-                rw [Vector.getElem_set_ne _ _ (by simp_all [Fin.val_ne_of_ne h])]
-                apply h2
-                exact Reachable.trans (reachable_of_edge (edge_of_low (h := O_root_def) O.1)) re1
-                exact re2
-termination_by O
-
-/-- `collect` is correct. -/
-theorem OBdd.collect_spec {O : OBdd n m} {j : Fin m} : Reachable O.1.heap O.1.root (node j) → j ∈ collect O := by
-  intro h
-  simp [collect]
-  apply collect_helper_spec
-  · intro i re ma
-    simp only [Fin.getElem_fin] at ma
-    rw [Vector.getElem_replicate _] at ma
-    contradiction
-  · assumption
-  · apply collect_spec' h
-    intro i re1 re2
-    simp only [Fin.getElem_fin, Vector.getElem_replicate]
-
-theorem OBdd.collect_helper_spec_reverse (O : OBdd n m) (r : Pointer m) I :
-    Reachable O.1.heap r O.1.root →
-    (∀ i ∈ I.2, Reachable O.1.heap r (node i)) →
-    ∀ i ∈ (collect_helper O I).2, Reachable O.1.heap r (node i) := by
-  intro h0 h1 i h2
-  cases h : O.1.root with
-  | terminal b =>
-    rw [collect_helper_terminal' O h] at h2
-    exact h1 i h2
-  | node j =>
-    rw [collect_helper_node' O h] at h2
-    split at h2
-    next ht =>
-      exact h1 i h2
-    next hf =>
-      cases List.instDecidableMemOfLawfulBEq i (j :: I.2) with
-      | isTrue htt =>
-        cases htt with
-        | head as    => convert h0; symm; assumption
-        | tail b hin => exact h1 i hin
-      | isFalse hff =>
-        cases List.instDecidableMemOfLawfulBEq i ((O.low h).collect_helper (I.1.set j true, j :: I.2)).2 with
-        | isFalse hhf =>
-          rw [← Bdd.high_heap_eq_heap (h := h)]
-          refine collect_helper_spec_reverse (O.high h) r _ ?_ ?_ i h2
-          · trans O.1.root
-            · exact h0
-            · exact reachable_of_edge (edge_of_high (h := h))
-          · intro i' hi'
-            simp only [high_heap_eq_heap]
-            rw [← low_heap_eq_heap (h := h)]
-            refine collect_helper_spec_reverse (O.low h) r _ ?_ ?_ i' hi'
-            · trans O.1.root
-              · exact h0
-              · exact reachable_of_edge (edge_of_low (h := h))
-            · intro i'' hi''
-              simp only at hi''
-              cases hi'' with
-              | head as     => simp only [low_heap_eq_heap]; convert h0; symm; assumption
-              | tail _ hi'' =>
-                simp only [low_heap_eq_heap]
-                exact h1 i'' hi''
-        | isTrue hht =>
-          rw [← low_heap_eq_heap (h := h)]
-          refine collect_helper_spec_reverse (O.low h) r _ ?_ ?_ i hht
-          · trans O.1.root
-            · exact h0
-            · exact reachable_of_edge (edge_of_low (h := h))
-          · intro i' hi'
-            simp only at hi'
-            cases hi' with
-            | head as    => simp only [low_heap_eq_heap]; convert h0; symm; assumption
-            | tail _ hi' =>
-              simp only [low_heap_eq_heap]
-              exact h1 i' hi'
-termination_by O
-
-theorem OBdd.collect_spec_reverse {O : OBdd n m} {j : Fin m} : j ∈ collect O → Reachable O.1.heap O.1.root (node j) := by
-  intro h
-  simp only [collect] at h
-  apply collect_helper_spec_reverse O O.1.root (Vector.replicate m false, []) (Relation.ReflTransGen.refl)
-  · simp
-  · assumption
-
-theorem OBdd.collect_helper_nodup {I : Vector Bool m × List (Fin m)} {O : OBdd n m} :
-    (∀ i ∈ I.2, I.1[i] = true) ∧ I.2.Nodup →
-    (∀ i ∈ (collect_helper O I).2, (collect_helper O I).1[i] = true) ∧ (collect_helper O I).2.Nodup := by
-  intro h
-  cases O_root_def : O.1.root with
-  | terminal b => simpa [collect_helper_terminal' O O_root_def]
-  | node     j =>
-    rw [collect_helper_node' O O_root_def]
-    split
-    next heq => assumption
-    next heq =>
-      apply collect_helper_nodup
-      apply collect_helper_nodup
-      simp only [List.mem_cons, forall_eq_or_imp, true_and]
-      constructor
-      · constructor
-        · simp
-        · intro i hi
-          cases decEq j i with
-          | isFalse hf =>
-            simp only [Fin.getElem_fin]
-            rw [Vector.getElem_set_ne _ _ (by simp_all [Fin.val_ne_of_ne hf])]
-            exact h.1 i hi
-          | isTrue  ht => simp_all
-      · constructor
-        · contrapose heq
-          simp_all
-        · exact h.2
-termination_by O
-
-theorem OBdd.mem_collect_iff_reachable {O : OBdd n m} {j : Fin m} : j ∈ collect O ↔ Reachable O.1.heap O.1.root (node j) := ⟨collect_spec_reverse, collect_spec⟩
-
-theorem OBdd.collect_nodup {O : OBdd n m} : (collect O).Nodup := by
-  simp only [collect]
-  exact (collect_helper_nodup (by simp)).2
-
-def OBdd.numPointers : OBdd n m → Nat := List.length ∘ collect
-
-lemma isTerminal_iff_numPointer_eq_zero {n m} {O : OBdd n m} : O.numPointers = 0 ↔ O.isTerminal := by
-  constructor
-  · intro h
-    simp only [OBdd.numPointers, Function.comp_apply, List.length_eq_zero_iff] at h
-    cases O_root_def : O.1.root with
-    | terminal b => use b
-    | node j =>
-      have := OBdd.collect_spec (j := j) (by rw [O_root_def]; exact Relation.ReflTransGen.refl)
-      rw [h] at this
-      contradiction
-  · rintro ⟨b, hb⟩
-    simp only [OBdd.numPointers, Function.comp_apply, List.length_eq_zero_iff, OBdd.collect]
-    rw [OBdd.collect_helper_terminal']
-    assumption
-
 lemma not_isTerminal_of_root_eq_node {n m} {j} {O : OBdd n m} (h : O.1.root = node j) : ¬ O.isTerminal := by
   rintro ⟨b, hb⟩
   rw [h] at hb
   contradiction
-
-def Bool_of_numPointer_eq_zero {n m} (O : OBdd n m) (h : O.numPointers = 0) : Bool :=
-  match O_root_def : O.1.root with
-  | terminal b => b
-  | node _ => False.elim (not_isTerminal_of_root_eq_node O_root_def (isTerminal_iff_numPointer_eq_zero.mp h))
 
 def OBdd.OReachable {n m} := Relation.ReflTransGen (@OEdge n m)
 
@@ -1618,22 +1139,6 @@ lemma OBdd.sub_eq_of_isTerminal {n m} {O : OBdd n m} (S : O.SubBdd) : O.isTermin
   | inl hl => assumption
   | inr hr =>
     rcases (Relation.transGen_swap.mp hr) with e | ⟨_, e⟩ <;> exact False.elim (not_OEdge_of_isTerminal h e)
-
-lemma OBdd.numPointers_gt_zero_of_Sub_root_eq_node {n m} {j} {O : OBdd n m} (S : O.SubBdd) : S.1.1.root = node j → O.numPointers > 0 := by
-  contrapose
-  simp only [gt_iff_lt, not_lt, nonpos_iff_eq_zero]
-  intro h
-  have := sub_eq_of_isTerminal S (isTerminal_iff_numPointer_eq_zero.mp h)
-  rw [this]
-  rcases isTerminal_iff_numPointer_eq_zero.mp h with ⟨b, hb⟩
-  rw [hb]
-  simp
-
-instance OBdd.instNeZeroNumPointers {n m} {j} {O : OBdd n m} (S : O.SubBdd) : S.1.1.root = node j → NeZero O.numPointers := by
-  intro h
-  have := numPointers_gt_zero_of_Sub_root_eq_node S h
-  constructor
-  linarith
 
 @[simp]
 def Bdd.lift_node : n ≤ n' → Node n m → Node n' m := fun h N ↦ ⟨⟨N.var.1, by exact Fin.val_lt_of_le N.var h⟩, N.low, N.high⟩
@@ -1867,7 +1372,7 @@ lemma OBdd.card_RelevantPointer_le {O : OBdd n m} : Fintype.card O.1.RelevantPoi
     | node i => simp [emb] at h; simp_rw [h]
     | terminal b => simp [emb] at h
 
-lemma OBdd.numPointers_terminal {O : OBdd n m} : O.isTerminal → Fintype.card O.1.RelevantPointer = 1 := by
+lemma OBdd.card_relevantPointer_eq_one_of_isTerminal {O : OBdd n m} : O.isTerminal → Fintype.card O.1.RelevantPointer = 1 := by
   intro h
   refine Fintype.card_eq_one_iff.mpr ?_
   rcases h with ⟨b, hb⟩
@@ -2034,22 +1539,6 @@ lemma OBdd.card_reachable_node {O : OBdd n m} (h : O.1.root = node j) :
     · apply instFintypeEitherRelevantPointer (O.low h) (O.high h); simp
     · simp
   · exact Fintype.subtypeEq O.1.root
-
-lemma OBdd.numPointers_spec {O : OBdd n m} : O.numPointers = Fintype.card { j // Reachable O.1.heap O.1.root (node j) } := by
-  simp only [numPointers, Function.comp_apply]
-  simp_rw [Fintype.card, Finset.univ]
-  have : O.collect.length = (Multiset.ofList O.collect).card := by rfl
-  rw [this]
-  refine Eq.symm (Finset.card_eq_of_bijective (fun i hi ↦ ⟨O.collect.get ⟨i, hi⟩, by simp; exact collect_spec_reverse (List.getElem_mem hi)⟩) ?_ ?_ ?_)
-  · rintro ⟨j, hj⟩ h
-    simp only [Subtype.mk.injEq, Multiset.coe_card]
-    exact List.mem_iff_getElem.mp (collect_spec hj)
-  · rintro i hi
-    simp only [List.get_eq_getElem]
-    apply Fintype.complete
-  · intro i j hi hj heq
-    simp only [List.get_eq_getElem, Subtype.mk.injEq] at heq
-    exact (List.Nodup.getElem_inj_iff collect_nodup).mp heq
 
 lemma Bdd.ordered_of_low_high_ordered {B : Bdd n m} (h : B.root = node j):
     (B.low h).Ordered → B.var < (B.low h).var → (B.high h).Ordered → B.var < (B.high h).var → Ordered B := by
@@ -2627,102 +2116,6 @@ instance OBdd.instDecidableUsesVar {O : OBdd n m} : DecidablePred O.1.usesVar :=
   intro i
   simp [usesVar]
   infer_instance
-
-lemma OBdd.numPointers_node_le {O : OBdd n m} {h : O.1.root = node j} :
-    O.numPointers ≤ 1 + (O.low h).numPointers + (O.high h).numPointers := by
-  rw [numPointers_spec]
-  rw [numPointers_spec]
-  rw [numPointers_spec]
-  rw [show 1 = Fintype.card {j' // j' = j} by simp]
-  rw [add_assoc]
-  rw [← Fintype.card_sum]
-  rw [← Fintype.card_sum]
-  refine Fintype.card_le_of_embedding ⟨?_, ?_⟩
-  · exact
-    fun ⟨j', hj'⟩ ↦ match decEq j' j with
-      | isTrue ht => .inl ⟨j', ht⟩
-      | isFalse hf => .inr (
-        match instDecidableReachable (O.low h) (node j') with
-        | isTrue htt => .inl ⟨j', htt⟩
-        | isFalse hff => .inr ⟨j', by
-          apply reachable_or_eq_low_high at hj'
-          cases hj' with
-          | inl hh => simp_all
-          | inr hh =>
-            rcases hh with ⟨jj, hjj1, hjj2⟩
-            have : node j = node jj := by rw [← h, hjj1]
-            injection this with that
-            subst that
-            cases hjj2 with
-            | inl hhh => simp_all
-            | inr hhh => exact hhh
-          ⟩
-        )
-  · intro x y hxy
-    simp only [low_heap_eq_heap, high_heap_eq_heap] at hxy
-    split at hxy
-    next =>
-      split at hxy <;> (refine Subtype.eq ?_; simp_all)
-    next =>
-      split at hxy <;>
-      (next =>
-        split at hxy
-        next => simp_all
-        next => split at hxy <;> (refine Subtype.eq ?_; simp_all))
-
-lemma OBdd.numPointers_le' {O : OBdd n m} : O.numPointers ≤ 2 ^ (n - O.1.var.1) - 1 := by
-  cases O_root_def : O.1.root with
-  | terminal b => simp [isTerminal_iff_numPointer_eq_zero.mpr ⟨b, O_root_def⟩]
-  | node j =>
-    calc _
-      _ ≤ 1 + (O.low O_root_def).numPointers + (O.high O_root_def).numPointers := numPointers_node_le
-      _ ≤ 1 + (2 ^ (n - (O.low O_root_def).1.var.1) - 1) + (2 ^ (n - (O.high O_root_def).1.var.1) - 1) := by
-        have := numPointers_le' (O := O.low O_root_def)
-        have := numPointers_le' (O := O.high O_root_def)
-        omega
-      _ ≤ 1 + (2 ^ (n - (O.1.var.1 + 1)) - 1) + (2 ^ (n - (O.high O_root_def).1.var.1) - 1) := by
-        simp only [Nat.succ_eq_add_one, low_heap_eq_heap, add_le_add_iff_right, add_le_add_iff_left, tsub_le_iff_right]
-        rw [Nat.sub_add_cancel (by exact Nat.one_le_two_pow)]
-        apply pow_le_pow_right' (by simp)
-        have := var_lt_low_var (h := O_root_def)
-        simp only [var] at this
-        omega
-      _ ≤ 1 + (2 ^ (n - (O.1.var.1 + 1)) - 1) + (2 ^ (n - (O.1.var.1 + 1)) - 1) := by
-        simp only [Nat.succ_eq_add_one, low_heap_eq_heap, add_le_add_iff_right, add_le_add_iff_left, tsub_le_iff_right]
-        rw [Nat.sub_add_cancel (by exact Nat.one_le_two_pow)]
-        apply pow_le_pow_right' (by simp)
-        have := var_lt_high_var (h := O_root_def)
-        simp only [var] at this
-        omega
-      _ ≤ 1 + (2 ^ ((n - O.1.var.1) - 1) - 1) + (2 ^ (n - (O.1.var.1 + 1)) - 1) := by
-        simp only [Nat.succ_eq_add_one, add_le_add_iff_right, add_le_add_iff_left, tsub_le_iff_right]
-        rw [Nat.sub_add_cancel (by exact Nat.one_le_two_pow)]
-        apply pow_le_pow_right' (by simp)
-        omega
-      _ ≤ 1 + (2 ^ ((n - O.1.var.1) - 1) - 1) + (2 ^ ((n - O.1.var.1) - 1) - 1) := by
-        simp only [Nat.succ_eq_add_one, add_le_add_iff_right, add_le_add_iff_left, tsub_le_iff_right]
-        rw [Nat.sub_add_cancel (by exact Nat.one_le_two_pow)]
-        apply pow_le_pow_right' (by simp)
-        omega
-      _ ≤ 2 ^ ((n - O.1.var.1) - 1) + 2 ^ ((n - O.1.var.1) - 1) - 1 := by
-        simp only [Nat.succ_eq_add_one]
-        have := Nat.one_le_two_pow (n := ((n - O.1.var.1) - 1))
-        omega
-      _ ≤ 2*2 ^ ((n - O.1.var.1) - 1) - 1 := by omega
-      _ ≤ 2 ^ (n - O.1.var.1) - 1 := by
-        refine Nat.sub_le_sub_right ?_ 1
-        apply le_of_eq
-        refine mul_pow_sub_one ?_ 2
-        simp [O_root_def]
-        omega
-termination_by O
-
-lemma OBdd.numPointers_le {O : OBdd n m} : O.numPointers ≤ 2 ^ n - 1 := by
-  trans 2 ^ (n - O.1.var.1) - 1
-  · exact OBdd.numPointers_le'
-  · simp only [Nat.succ_eq_add_one, tsub_le_iff_right]
-    rw [Nat.sub_add_cancel (by exact Nat.one_le_two_pow)]
-    apply Nat.pow_le_pow_right <;> omega
 
 def OBdd.evaluate' (O : OBdd n m) : Vector Bool n → Bool := fun I ↦
   match h : O.1.root with
