Bdd/Collect.lean
@@ -1,0 +1,467 @@
+
+import Bdd.Basic
+
+namespace Collect
+
+private def collect_helper (O : OBdd n m) : Vector Bool m × List (Fin m) → Vector Bool m × List (Fin m) :=
+  match h : O.1.root with
+  | .terminal _ => id
+  | .node j =>
+    fun I ↦ if I.1.get j then I else collect_helper (O.high h) (collect_helper (O.low h) ⟨I.1.set j true, j :: I.2⟩)
+termination_by O
+
+/-- Return a list of all reachable node indices. -/
+def collect (O : OBdd n m) : List (Fin m) := (collect_helper O ⟨Vector.replicate m false, []⟩).2
+
+private lemma collect_helper_terminal {v : Vector (Node n m) m} {h : Bdd.Ordered {heap := v, root := .terminal b}} :
+    collect_helper ⟨{heap := v, root := .terminal b}, h⟩ I = I := by
+  conv =>
+    lhs
+    unfold collect_helper
+  congr
+
+private lemma collect_helper_terminal' {O : OBdd n m} (h : O.1.root = .terminal b) :
+    collect_helper O I = I := by
+  rcases O with ⟨⟨M, r⟩, o⟩
+  simp only at h
+  have := collect_helper_terminal (h := (show Bdd.Ordered {heap := M, root := .terminal b} by simp_rw [← h]; exact o)) (I := I)
+  simp_rw [h]
+  assumption
+
+lemma collect_terminal {O : OBdd n m} (h : O.1.root = .terminal b) :
+    collect O = [] := by
+  simp only [collect, collect_helper_terminal' h]
+
+private lemma collect_helper_node {v : Vector (Node n m) m} {h : Bdd.Ordered {heap := v, root := .node j}} :
+    collect_helper ⟨{heap := v, root := .node j}, h⟩ I =
+      if I.1[j]
+      then I
+      else collect_helper ⟨⟨v, v[j].high⟩, Bdd.ordered_of_relevant ⟨⟨v, .node j⟩, h⟩ ⟨v[j].high, Bdd.reachable_of_edge (Edge.high rfl)⟩⟩
+                          (collect_helper ⟨{heap := v, root := v[j].low}, Bdd.ordered_of_relevant ⟨{heap := v, root := .node j}, h⟩ ⟨v[j].low, Bdd.reachable_of_edge (Edge.low rfl)⟩⟩
+                                          ⟨I.1.set j true, j :: I.2⟩) := by
+  conv =>
+    lhs
+    unfold collect_helper
+  congr
+
+private lemma collect_helper_node' (O : OBdd n m) {j : Fin m} (h : O.1.root = .node j) :
+    collect_helper O I = if I.1[j] then I else collect_helper (O.high h) (collect_helper (O.low h) ⟨I.1.set j true, j :: I.2⟩) := by
+  rcases O with ⟨⟨M, r⟩, o⟩
+  simp only at h
+  have := collect_helper_node (h := (show Bdd.Ordered {heap := M, root := .node j} by simp_rw [← h]; exact o)) (I := I)
+  simp_rw [h]
+  assumption
+
+private theorem collect_helper_retains_found {O : OBdd n m} {I : Vector Bool m × List (Fin m)} :
+    j ∈ I.2 → j ∈ (collect_helper O I).2 := by
+  intro h
+  cases O_root_def : O.1.root with
+  | terminal b =>
+    rw [collect_helper_terminal' O_root_def]
+    assumption
+  | node i =>
+    rw [collect_helper_node' O O_root_def]
+    cases I.1[i]
+    case true  => simpa
+    case false =>
+      simp only [Bool.false_eq_true, ↓reduceIte]
+      have : j ∈ (collect_helper (O.low O_root_def) (I.1.set i true, i :: I.2)).2 := by
+        apply collect_helper_retains_found
+        simp only []
+        cases decEq j i with
+        | isFalse hf => right; assumption
+        | isTrue ht => rw [ht]; left
+      exact collect_helper_retains_found this
+termination_by O
+
+private theorem collect_helper_retains_marked {O : OBdd n m} {I : Vector Bool m × List (Fin m)} {j : Fin m}:
+    I.1[j] = true → (collect_helper O I).1[j] = true := by
+  intro h
+  cases O_root_def : O.1.root with
+  | terminal b =>
+    rw [collect_helper_terminal' O_root_def]
+    assumption
+  | node i =>
+    rw [collect_helper_node' O O_root_def]
+    cases I.1[i]
+    case true  => simpa
+    case false =>
+      simp only [Bool.false_eq_true, ↓reduceIte]
+      have : (collect_helper (O.low O_root_def) (I.1.set i true, i :: I.2)).1[j] = true := by
+        apply collect_helper_retains_marked
+        simp only []
+        cases decEq i j with
+        | isFalse hf =>
+          have : i.1 ≠ j.1 := by
+            exact Fin.val_ne_of_ne hf
+          simp only [Fin.getElem_fin]
+          rw [Vector.getElem_set_ne _ _ this]
+          assumption
+        | isTrue ht => rw [ht]; simp
+      exact collect_helper_retains_marked this
+termination_by O
+
+private theorem collect_helper_only_marks_reachable {j : Fin m} {O : OBdd n m} {I : Vector Bool m × List (Fin m)} :
+    I.1[j] = false → (collect_helper O I).1[j] = true → Pointer.Reachable O.1.heap O.1.root (.node j) := by
+  intro h1 h2
+  cases O_root_def : O.1.root with
+  | terminal b =>
+    rw [collect_helper_terminal' O_root_def, h1] at h2; contradiction
+  | node i =>
+    cases decEq i j with
+    | isTrue ht  => rw [ht]; exact Relation.ReflTransGen.refl
+    | isFalse hf =>
+      rw [collect_helper_node' O O_root_def] at h2
+      cases hh : I.1[i] with
+      | true =>
+        rw [hh] at h2
+        simp only [↓reduceIte] at h2
+        rw [h1] at h2
+        contradiction
+      | false =>
+        rw [hh] at h2
+        simp at h2
+        rw [← O_root_def]
+        cases hhh : (collect_helper (O.low O_root_def) (I.1.set i true, i :: I.2)).1[j] with
+        | false =>
+          have : Pointer.Reachable (O.high O_root_def).1.heap (O.high O_root_def).1.root (.node j) := by
+            apply collect_helper_only_marks_reachable (I := (collect_helper (O.low O_root_def) (I.1.set i true, i :: I.2)))
+            · assumption
+            · assumption
+          simp at this
+          trans (O.high O_root_def).1.root
+          · exact Bdd.reachable_of_edge (Bdd.edge_of_high (h := O_root_def) O.1)
+          · assumption
+        | true =>
+          have : Pointer.Reachable (O.low O_root_def).1.heap (O.low O_root_def).1.root (.node j) := by
+            apply collect_helper_only_marks_reachable (I := (I.1.set i true, i :: I.2))
+            · have : i.1 ≠ j.1 := by
+                exact Fin.val_ne_of_ne hf
+              simp only [Fin.getElem_fin]
+              rw [Vector.getElem_set_ne _ _ this]
+              assumption
+            · assumption
+          simp at this
+          trans (O.low O_root_def).1.root
+          · exact Bdd.reachable_of_edge (Bdd.edge_of_low (h := O_root_def) O.1)
+          · assumption
+termination_by O
+
+private theorem collect_helper_spec {O : OBdd n m} :
+    (∀ i, (Pointer.Reachable O.1.heap O.1.root (.node i) → I.1[i] = true → i ∈ I.2)) →
+    ∀ i, (Pointer.Reachable O.1.heap O.1.root (.node i) → (collect_helper O I).1[i] → i ∈ (collect_helper O I).2) := by
+  intro h j re ma
+  cases O_root_def : O.1.root with
+  | terminal b =>
+    have : (⟨.node j, re⟩ : O.1.RelevantPointer).1  = .terminal b := by
+      apply Bdd.eq_terminal_of_relevant
+      rw [← O_root_def]
+    contradiction
+  | node k =>
+    rw [collect_helper_node' O O_root_def] at ma
+    rw [collect_helper_node' O O_root_def]
+    cases hh : I.1[k] with
+    | true =>
+      rw [hh] at ma
+      simp at ma
+      simp
+      exact h j re ma
+    | false =>
+      rw [hh] at ma
+      simp at ma
+      simp
+      cases decEq k j with
+      | isTrue hht =>
+        apply collect_helper_retains_found
+        apply collect_helper_retains_found
+        rw [hht]
+        left
+      | isFalse hhf =>
+        cases hhh : I.1[j] with
+        | true =>
+          apply collect_helper_retains_found
+          apply collect_helper_retains_found
+          right
+          apply h <;> assumption
+        | false=>
+          cases hhhh : (collect_helper (O.low O_root_def) (I.1.set k true, k :: I.2)).1[j] with
+          | true =>
+            have : j ∈ (collect_helper (O.low O_root_def) (I.1.set k true, k :: I.2)).2 := by
+              apply collect_helper_spec
+              · intro i' re' ma'
+                simp at ma'
+                simp at re'
+                simp only
+                cases decEq k i' with
+                | isFalse hff =>
+                  rw [Vector.getElem_set_ne _ _ (by simp_all [Fin.val_ne_of_ne hff])] at ma'
+                  right
+                  apply h
+                  exact Pointer.Reachable.trans (Bdd.reachable_of_edge (Bdd.edge_of_low (h := O_root_def) O.1)) re'
+                  exact ma'
+                | isTrue  htt => rw [htt]; left
+              · have : (I.1.set k true, k :: I.2).1[j] = false := by
+                  simp only [Fin.getElem_fin]
+                  rw [Vector.getElem_set_ne _ _ (by simp_all [Fin.val_ne_of_ne hhf])]
+                  exact hhh
+                apply collect_helper_only_marks_reachable this hhhh
+              · exact hhhh
+            apply collect_helper_retains_found this
+          | false=>
+            apply collect_helper_spec
+            · intro i' re' ma'
+              simp at ma' re'
+              have := h i' (Pointer.Reachable.trans (Bdd.reachable_of_edge (Bdd.edge_of_high (h := O_root_def) O.1)) re')
+              cases hhhhh : I.1[i'] with
+              | true =>
+                apply this at hhhhh
+                have : i' ∈ (I.1.set k true, k :: I.2).2 := by simp only; right; exact hhhhh
+                apply collect_helper_retains_found this
+              | false=>
+                cases decEq k i' with
+                | isTrue hhtt =>
+                  apply collect_helper_retains_found
+                  rw [hhtt]
+                  left
+                | isFalse hhff =>
+                  have that : (I.1.set k true, k :: I.2).1[i'] = false := by
+                    simp only [Fin.getElem_fin]
+                    rw [Vector.getElem_set_ne _ _ (by simp_all [Fin.val_ne_of_ne hhff])]
+                    exact hhhhh
+                  apply collect_helper_spec
+                  · intro i'' re'' ma''
+                    simp at ma''
+                    simp at re''
+                    simp only
+                    cases decEq k i'' with
+                    | isFalse hfff =>
+                      rw [Vector.getElem_set_ne _ _ (by simp_all [Fin.val_ne_of_ne hfff])] at ma''
+                      right
+                      apply h
+                      exact Pointer.Reachable.trans (Bdd.reachable_of_edge (Bdd.edge_of_low (h := O_root_def) O.1)) re''
+                      exact ma''
+                    | isTrue  htt => rw [htt]; left
+                  · apply collect_helper_only_marks_reachable that ma'
+                  · exact ma'
+            · apply collect_helper_only_marks_reachable hhhh ma
+            · assumption
+termination_by O
+
+private lemma collect_spec' {O : OBdd n m} {j : Fin m} {I : Vector Bool m × List (Fin m)} :
+    Pointer.Reachable O.1.heap O.1.root (.node j) →
+    (∀ i, (Pointer.Reachable O.1.heap O.1.root (.node i) → Pointer.Reachable O.1.heap (.node i) (.node j) → I.1[i] = false)) →
+    (collect_helper O I).1[j] = true := by
+  intro h1 h2
+  cases O_root_def : O.1.root with
+  | terminal b =>
+    have : (⟨.node j, h1⟩ : O.1.RelevantPointer).1  = .terminal b := by
+      apply Bdd.eq_terminal_of_relevant
+      rw [← O_root_def]
+    contradiction
+  | node i =>
+    rw [collect_helper_node' O O_root_def]
+    have : I.1[i] = false := by
+      apply h2 i
+      · rw [← O_root_def]
+        exact Relation.ReflTransGen.refl
+      · rw [← O_root_def]
+        exact h1
+    rw [this]
+    simp only [Bool.false_eq_true, ↓reduceIte]
+    cases decEq i j with
+    | isTrue h =>
+      apply collect_helper_retains_marked
+      apply collect_helper_retains_marked
+      rw [h]
+      simp
+    | isFalse hij =>
+      cases Pointer.instDecidableReachable (O.low O_root_def) (.node j) with
+      | isTrue ht  =>
+        apply collect_helper_retains_marked
+        apply collect_spec'
+        · exact ht
+        · intro i' re1 re2
+          simp only
+          cases decEq i i' with
+          | isTrue h =>
+            exfalso
+            apply OBdd.not_oedge_reachable (oedge_of_low (h := O_root_def))
+            rw [← h] at re1
+            rw [O_root_def]
+            exact re1
+          | isFalse h =>
+            simp only [Fin.getElem_fin]
+            rw [Vector.getElem_set_ne _ _ (by simp_all [Fin.val_ne_of_ne h])]
+            apply h2
+            exact Pointer.Reachable.trans (Bdd.reachable_of_edge (Bdd.edge_of_low (h := O_root_def) O.1)) re1
+            exact re2
+      | isFalse hf =>
+        apply collect_spec'
+        · cases (OBdd.reachable_or_eq_low_high (p := .node j) h1) with
+        | inl h => rw [O_root_def] at h; simp at h; contradiction
+        | inr h =>
+          rcases h with ⟨j', h', d⟩
+          have same : i = j' := by rw [O_root_def] at h'; simp at h'; assumption
+          subst same
+          cases d with
+          | inl => contradiction
+          | inr => assumption
+        · intro i' re ma
+          contrapose! hf
+          simp only [Bool.not_eq_false] at hf
+          apply collect_helper_only_marks_reachable (I := (I.1.set i true, i :: I.2))
+          simp only [Fin.getElem_fin]
+          rw [Vector.getElem_set_ne _ _ (by simp_all [Fin.val_ne_of_ne hij])]
+          apply h2
+          · exact Pointer.Reachable.trans (Bdd.reachable_of_edge (Bdd.edge_of_high (h := O_root_def) O.1)) (Pointer.Reachable.trans re ma)
+          · exact Relation.ReflTransGen.refl
+          · apply collect_spec'
+            · have that : Pointer.Reachable (O.low O_root_def).1.heap (O.low O_root_def).1.root (.node i') := by
+                apply collect_helper_only_marks_reachable (I := (I.1.set i true, i :: I.2))
+                · cases decEq i i' with
+                  | isFalse hff =>
+                    simp only [Fin.getElem_fin]
+                    rw [Vector.getElem_set_ne _ _ (by simp_all [Fin.val_ne_of_ne hff])]
+                    apply h2 i' (Pointer.Reachable.trans (Bdd.reachable_of_edge (Bdd.edge_of_high (h := O_root_def) O.1)) re) ma
+                  | isTrue htt =>
+                    exfalso
+                    apply OBdd.not_oedge_reachable (oedge_of_high (h := O_root_def))
+                    rw [htt] at O_root_def
+                    rw [O_root_def]
+                    exact re
+                · assumption
+              exact Pointer.Reachable.trans that ma
+            · intro i'' re1 re2
+              simp only
+              cases decEq i i'' with
+              | isTrue h =>
+                rw [← h] at re1
+                exfalso
+                apply OBdd.not_oedge_reachable (oedge_of_low (h := O_root_def))
+                rw [O_root_def]
+                exact re1
+              | isFalse h =>
+                simp only [Fin.getElem_fin]
+                rw [Vector.getElem_set_ne _ _ (by simp_all [Fin.val_ne_of_ne h])]
+                apply h2
+                exact Pointer.Reachable.trans (Bdd.reachable_of_edge (Bdd.edge_of_low (h := O_root_def) O.1)) re1
+                exact re2
+termination_by O
+
+/-- `collect` is correct. -/
+theorem collect_spec {O : OBdd n m} {j : Fin m} : Pointer.Reachable O.1.heap O.1.root (.node j) → j ∈ collect O := by
+  intro h
+  simp [collect]
+  apply collect_helper_spec
+  · intro i re ma
+    simp only [Fin.getElem_fin] at ma
+    rw [Vector.getElem_replicate _] at ma
+    contradiction
+  · assumption
+  · apply collect_spec' h
+    intro i re1 re2
+    simp only [Fin.getElem_fin, Vector.getElem_replicate]
+
+private theorem collect_helper_spec_reverse (O : OBdd n m) (r : Pointer m) I :
+    Pointer.Reachable O.1.heap r O.1.root →
+    (∀ i ∈ I.2, Pointer.Reachable O.1.heap r (.node i)) →
+    ∀ i ∈ (collect_helper O I).2, Pointer.Reachable O.1.heap r (.node i) := by
+  intro h0 h1 i h2
+  cases h : O.1.root with
+  | terminal b =>
+    rw [collect_helper_terminal' h] at h2
+    exact h1 i h2
+  | node j =>
+    rw [collect_helper_node' O h] at h2
+    split at h2
+    next ht =>
+      exact h1 i h2
+    next hf =>
+      cases List.instDecidableMemOfLawfulBEq i (j :: I.2) with
+      | isTrue htt =>
+        cases htt with
+        | head as    => convert h0; symm; assumption
+        | tail b hin => exact h1 i hin
+      | isFalse hff =>
+        cases List.instDecidableMemOfLawfulBEq i (collect_helper (O.low h) (I.1.set j true, j :: I.2)).2 with
+        | isFalse hhf =>
+          rw [← Bdd.high_heap_eq_heap (h := h)]
+          refine collect_helper_spec_reverse (O.high h) r _ ?_ ?_ i h2
+          · trans O.1.root
+            · exact h0
+            · exact Bdd.reachable_of_edge (Bdd.edge_of_high (h := h))
+          · intro i' hi'
+            simp only [OBdd.high_heap_eq_heap]
+            rw [← OBdd.low_heap_eq_heap (h := h)]
+            refine collect_helper_spec_reverse (O.low h) r _ ?_ ?_ i' hi'
+            · trans O.1.root
+              · exact h0
+              · exact Bdd.reachable_of_edge (Bdd.edge_of_low (h := h))
+            · intro i'' hi''
+              simp only at hi''
+              cases hi'' with
+              | head as     => simp only [OBdd.low_heap_eq_heap]; convert h0; symm; assumption
+              | tail _ hi'' =>
+                simp only [OBdd.low_heap_eq_heap]
+                exact h1 i'' hi''
+        | isTrue hht =>
+          rw [← OBdd.low_heap_eq_heap (h := h)]
+          refine collect_helper_spec_reverse (O.low h) r _ ?_ ?_ i hht
+          · trans O.1.root
+            · exact h0
+            · exact OBdd.reachable_of_edge (Bdd.edge_of_low (h := h))
+          · intro i' hi'
+            simp only at hi'
+            cases hi' with
+            | head as    => simp only [OBdd.low_heap_eq_heap]; convert h0; symm; assumption
+            | tail _ hi' =>
+              simp only [OBdd.low_heap_eq_heap]
+              exact h1 i' hi'
+termination_by O
+
+theorem collect_spec_reverse {O : OBdd n m} {j : Fin m} :
+    j ∈ collect O → Pointer.Reachable O.1.heap O.1.root (.node j) := by
+  intro h
+  simp only [collect] at h
+  apply collect_helper_spec_reverse O O.1.root (Vector.replicate m false, []) (Relation.ReflTransGen.refl)
+  · simp
+  · assumption
+
+private theorem collect_helper_nodup {I : Vector Bool m × List (Fin m)} {O : OBdd n m} :
+    (∀ i ∈ I.2, I.1[i] = true) ∧ I.2.Nodup →
+    (∀ i ∈ (collect_helper O I).2, (collect_helper O I).1[i] = true) ∧ (collect_helper O I).2.Nodup := by
+  intro h
+  cases O_root_def : O.1.root with
+  | terminal b => simpa [collect_helper_terminal' O_root_def]
+  | node     j =>
+    rw [collect_helper_node' O O_root_def]
+    split
+    next heq => assumption
+    next heq =>
+      apply collect_helper_nodup
+      apply collect_helper_nodup
+      simp only [List.mem_cons, forall_eq_or_imp, true_and]
+      constructor
+      · constructor
+        · simp
+        · intro i hi
+          cases decEq j i with
+          | isFalse hf =>
+            simp only [Fin.getElem_fin]
+            rw [Vector.getElem_set_ne _ _ (by simp_all [Fin.val_ne_of_ne hf])]
+            exact h.1 i hi
+          | isTrue  ht => simp_all
+      · constructor
+        · contrapose heq
+          simp_all
+        · exact h.2
+termination_by O
+
+theorem mem_collect_iff_reachable {O : OBdd n m} {j : Fin m} :
+    j ∈ collect O ↔ Pointer.Reachable O.1.heap O.1.root (.node j) := ⟨collect_spec_reverse, collect_spec⟩
+
+theorem collect_nodup {O : OBdd n m} : (collect O).Nodup := by
+  simp only [collect]
+  exact (collect_helper_nodup (by simp)).2
+
+end Collect
