Bdd/Compactify.lean
@@ -1,10 +1,11 @@
 import Bdd.Basic
+import Bdd.Size
 
 open Pointer
 
 namespace Compactify
 
-def compactify_helper {n m : Nat} (O : OBdd n m) (S : O.SubBdd) (ids : Vector (Option (Fin O.numPointers)) m) (nid : Fin O.numPointers) (new : Vector (Node n O.numPointers) O.numPointers) : Vector (Option (Fin O.numPointers)) m × Fin O.numPointers × Vector (Node n O.numPointers) O.numPointers × Pointer O.numPointers :=
+def compactify_helper {n m : Nat} (O : OBdd n m) (S : O.SubBdd) (ids : Vector (Option (Fin (Size.size O))) m) (nid : Fin (Size.size O)) (new : Vector (Node n (Size.size O)) (Size.size O)) : Vector (Option (Fin (Size.size O))) m × Fin (Size.size O) × Vector (Node n (Size.size O)) (Size.size O) × Pointer (Size.size O) :=
   match S_root_def : S.1.1.root with
     | terminal b => ⟨ ids, nid, new, terminal b ⟩
     | node j =>
@@ -12,25 +13,25 @@ def compactify_helper {n m : Nat} (O : OBdd n m) (S : O.SubBdd) (ids : Vector (O
       | none =>
         let ⟨ ids1, nid1, new1, l ⟩ := compactify_helper O (S.low  S_root_def) ids  nid  new
         let ⟨ ids2, nid2, new2, h ⟩ := compactify_helper O (S.high S_root_def) ids1 nid1 new1
-        have : NeZero O.numPointers := OBdd.instNeZeroNumPointers S S_root_def
+        have : NeZero (Size.size O) := Size.instNeZeroSize S S_root_def
         ⟨ ids2.set j (some nid2), nid2 + 1, new2.set nid2 ⟨O.1.heap[j].var, l, h⟩, node nid2 ⟩
       | some j' => ⟨ ids, nid, new, node j' ⟩
 termination_by S.1
 
-def compactify' {n m : Nat} (O : OBdd n m) : Bdd n O.numPointers :=
+def compactify' {n m : Nat} (O : OBdd n m) : Bdd n (Size.size O) :=
   match O_root_def : O.1.root with
   | terminal b =>
-    have := isTerminal_iff_numPointer_eq_zero.mpr ⟨b, O_root_def⟩
-    ⟨this ▸ Vector.emptyWithCapacity 0, terminal (Bool_of_numPointer_eq_zero O this)⟩
+    have := Size.isTerminal_iff_size_eq_zero.mpr ⟨b, O_root_def⟩
+    ⟨this ▸ Vector.emptyWithCapacity 0, terminal (Size.bool_of_size_eq_zero O this)⟩
   | node j =>
-    let ⟨ ids, nid, new, r ⟩ := compactify_helper O O.toSubBdd (Vector.replicate m none) ⟨0, OBdd.numPointers_gt_zero_of_Sub_root_eq_node (O.toSubBdd) O_root_def⟩ (Vector.replicate O.numPointers ⟨O.1.heap[j].var, (terminal false), (terminal false)⟩)
+    let ⟨ ids, nid, new, r ⟩ := compactify_helper O O.toSubBdd (Vector.replicate m none) ⟨0, Size.size_gt_zero_of_Sub_root_eq_node (O.toSubBdd) O_root_def⟩ (Vector.replicate (Size.size O) ⟨O.1.heap[j].var, (terminal false), (terminal false)⟩)
     ⟨new, r⟩
 
 lemma compactify_helper_spec'
     (O : OBdd n m) (S : O.SubBdd)
-    (ids : Vector (Option (Fin O.numPointers)) m)
-    (nid : Fin O.numPointers)
-    (new : Vector (Node n O.numPointers) O.numPointers) :
+    (ids : Vector (Option (Fin (Size.size O))) m)
+    (nid : Fin (Size.size O))
+    (new : Vector (Node n (Size.size O)) (Size.size O)) :
     nid = Fintype.card {j // (ids.get j).isSome} →
     ( ∀ j j',
       ids.get j = some j' →
@@ -78,111 +79,6 @@ lemma compactify_helper_spec'
         simp_rw [this]
         rfl
 
--- lemma compactify_helper_spec {Proper Ordered_of_Proper} {n m : Nat}
---     (O : OBdd n m) (S : O.SubBdd) (ids : Vector (Option (Fin O.numPointers)) m) (nid : Fin O.numPointers) (new : Vector (Node n O.numPointers) O.numPointers) (hp : Proper new):
---     ( ∀ j j',
---       ids.get j = some j' →
---       ∃ (r : Reachable O.1.heap O.1.root (node j)),
---         OBdd.HSimilar ⟨⟨O.1.heap, node j⟩, Bdd.ordered_of_relevant O ⟨node j, r⟩⟩ ⟨⟨new, node j'⟩, Ordered_of_Proper hp⟩
---     ) →
---     let ⟨ ids1, nid1, new1, root ⟩ := compactify_helper O S ids nid new
---     ∃ (hp' : Proper new1),
---       (∀ j j',
---        ids1.get j = some j' →
---        ∃ (r : Reachable O.1.heap O.1.root (node j)),
---          OBdd.HSimilar ⟨⟨O.1.heap, node j⟩, Bdd.ordered_of_relevant O ⟨node j, r⟩⟩ ⟨⟨new1, node j'⟩, Ordered_of_Proper hp'⟩
---       ) ∧ OBdd.HSimilar S.1 ⟨⟨new1, root⟩, Ordered_of_Proper hp'⟩ := by
---   intro h
---   unfold compactify_helper
---   split
---   next ids2 nid2 new2 root heq =>
---     split at heq
---     next b heqq =>
---       simp only [Prod.mk.injEq] at heq
---       rcases heq with ⟨heq1, heq2, heq3, heq4⟩
---       rw [← heq3, ← heq1, ← heq4]
---       use hp
---       constructor
---       · exact h
---       · exact OBdd.HSimilar_of_terminal heqq rfl
---     next r heqq =>
---       split at heq
---       next heqqq =>
---         split at heq
---         next ids0 nid0 new0 lh heqqqq =>
---           split at heq
---           next ids1 nid1 new1 rh heqqqqq =>
---           simp only [Prod.mk.injEq] at heq
---           rcases heq with ⟨heq1, heq2, heq3, heq4⟩
---           have hp2 : Proper new2 := by
---             apply Proper_of_all_indices_RespectsOrder
---             intro j
---             nth_rw 2 [← heq3]
---             cases decEq nid1 j with
---             | isFalse hf =>
---               rw [Vec.get_set_of_ne' hf]
---               sorry
---             | isTrue ht =>
---               rw [ht, Vec.get_set_same']
---               sorry
---           sorry
---       next j heqqq => sorry
-  --     have hp' : Proper new1 := by
-  --       sorry
-  --     sorry
-  -- next b heq =>
-  --   constructor
-  --   · constructor
-  --     · exact h
-  --     · exact OBdd.HSimilar_of_terminal heq rfl
-  --   · simpa
-  -- next j heq =>
-  --   constructor
-  --   case w =>
-  --     split
-  --     next heqq =>
-  --       simp only
-  --       apply Proper_of_all_indices_RespectsOrder
-  --       intro i
-  --       sorry
-  --     next j' heqq => exact hp
-  --   case h =>
-  --     constructor
-  --     · intro jj j' hjj'
-  --       sorry
-  --     · sorry
-    -- · sorry
-    -- · constructor
-    --   · sorry
-    --   · constructor
-    --     case w =>
-    --       split
-    --       next heqq =>
-    --         simp only
-    --         apply Ordered_of_low_high_ordered
-    --         · rw [Vec.get_set_same']
-    --           simp only
-    --           suffices Bdd.Ordered ⟨(compactify_helper O (S.low heq) ids nid new).2.2.1, (compactify_helper O (S.low heq) ids nid new).2.2.2⟩ by
-    --             rintro ⟨x, hx⟩ ⟨y, hy⟩ hxy
-    --             simp only [RelevantEdge, Ordered] at hxy
-    --             simp only [Ordered] at hx hy
-    --             simp only [RelevantMayPrecede, MayPrecede]
-    --             sorry
-    --           rcases (compactify_helper_spec O (S.low heq) ids nid new h hp).2 with ⟨hhh, _⟩
-    --           exact hhh
-    --         · sorry
-    --         · sorry
-    --         · sorry
-    --       next j' heqq =>
-    --         exact (h j j' heqq).2.1
-    --     case h => sorry
-    -- split
-    -- next heqq =>
-    --   simp only
-    --   sorry
-    -- next j' heqq => exact h j j' heqq
-
-
 lemma compactify_ordered {n m : Nat} {O : OBdd n m} : (compactify' O).Ordered := by
   unfold compactify'
   split
@@ -190,8 +86,6 @@ lemma compactify_ordered {n m : Nat} {O : OBdd n m} : (compactify' O).Ordered :=
   next j heq =>
     split
     next x ids nid new root heqq => sorry
-
---theorem compactify_spec {n m : Nat} {O : OBdd n m} : O.Similar (compactify O) :=
 
 lemma compactify_preserves_reduced {O : OBdd n m} :
     OBdd.Reduced O → OBdd.Reduced ⟨(compactify' O), compactify_ordered⟩ := by
@@ -202,26 +96,3 @@ lemma compactify_evaluate {O : OBdd n m} :
   sorry
 
 end Compactify
--- #eval (example_not_reduced_bdd).numPointers
--- #eval (example_bdd).numPointers
-
--- #eval example_bdd
--- #eval! Compactify.compactify' example_bdd
--- theorem compactify_induction {n m : Nat} {O : OBdd n m} {motive : Bdd n O.numPointers → Prop}
---     (one : (h : O.numPointers = 0) → motive ⟨h ▸ Vec.nil, terminal (Bool_of_numPointer_eq_zero O h)⟩)
---     (two : ∀ (k : Nat), O.numPointers = k.succ → motive (compactify O)) :
---     motive (compactify O) := by
---   cases h : O.numPointers with
---   | zero =>
---     convert one h
---     · unfold compactify
---       simp
---     rw [compactify.]
---   | succ k => sorry
-
--- def compactify {n m : Nat} (O : OBdd n m) : Bdd n O.numPointers :=
---   match h : O.numPointers with
---   | 0 => ⟨Vec.nil, terminal (Bool_of_numPointer_eq_zero O h)⟩
---   | Nat.succ k =>
---     let ⟨ ids, nid, new, r ⟩ := compactify_helper O O.toSubBdd (Vec.replicate m none) ⟨0, by linarith⟩ (Vec.replicate O.numPointers ⟨(O.1.heap.get ⟨0, lt_of_le_of_lt (show 0 ≤ k by linarith) sorry⟩).var, (terminal false), (terminal false)⟩)
---     h ▸ ⟨new, r⟩
